src/graph_theory/path3.lean
@@ -6,28 +6,36 @@ namespace simple_graph
     | point : path x
     | step {y z : V} : path y -> G.adj y z -> path z
 
+    infix ` · `:50 := path.step
+
     namespace path
         open path
         variables {V : Type} {G : simple_graph V} {u v x y z : V} {e : edges G}
         variables {p : path G x y} {p' : path G y z} {h : G.adj y z} {h' : G.adj u x} {h'' : G.adj z v}
 
-        @[simp] def from_edge : G.adj x y -> path G x y := step point
+        @[simp] def cons (h : G.adj x y) : Π {z : V}, path G y z -> path G x z
+            | _ point    := point · h
+            | _ (p · h') := cons p · h'
 
-        @[simp] def cons : Π {z : V}, path G y z -> G.adj x y -> path G x z -- TODO: cons h p instead
-            | _ point h       := step point h
-            | _ (step p h') h := step (cons p h) h'
+        infixr ` :: ` := cons
 
         @[simp] def concat (p : path G x y) : Π {z : V}, path G y z -> path G x z
-            | _ point       := p
-            | _ (step p' h) := step (concat p') h
+            | _ point    := p
+            | _ (p' · h) := concat p' · h
 
-        def mem (z : V) (p : path G x y) : Prop           := path.rec (z=x) (λ _ u _ _ h, h ∨ z=u)           p
+        infix ` ++ ` := concat
+
+        @[simp] def mem (z : V) : Π {y : V}, path G x y -> Prop
+            | _ point   := z = x
+            | y (p · h) := mem p ∨ z = y
+
+        instance : has_mem V (path G x y) := ⟨λ z, mem z⟩
+
         def size        (p : path G x y) : ℕ              := path.rec 0     (λ _ _ _ _ l, l+1)               p
-        def rev         (p : path G x y) : path G y x    := path.rec point (λ _ _ _ h q, q.cons (G.symm h)) p
+        def rev         (p : path G x y) : path G y x     := path.rec point (λ _ _ _ h q, cons (G.symm h) q) p
         def edges       (p : path G x y) : list (edges G) := path.rec []    (λ _ _ _ d e, ⟨d⟩ :: e)          p
         def nodup       (p : path G x y) : Prop           := path.rec true  (λ _ u q _ e, e ∧ ¬(mem u q))    p
 
-        instance : has_mem    V (path G x y) := ⟨mem⟩
         instance : has_sizeof   (path G x y) := ⟨size⟩
 
         @[simp] lemma mem_point    :   u ∈ (@point _ G x) <-> u = x       := iff.rfl
@@ -36,24 +44,24 @@ namespace simple_graph
         @[simp] lemma edges_point  : edges (@point _ G x)  =  []          := rfl
         @[simp] lemma nodup_point  : nodup (@point _ G x)                 := trivial
 
-        @[simp] lemma mem_step    :           u ∈ p.step h <-> u ∈ p ∨ u = z          := iff.rfl
-        @[simp] lemma size_step   :        (p.step h).size  =  p.size + 1             := rfl
-        @[simp] lemma rev_step    :         rev (p.step h)  =  cons p.rev (G.symm h)  := rfl
-        @[simp] lemma edges_step  :       edges (p.step h)  =  ⟨h⟩ :: edges p         := rfl
-        @[simp] lemma nodup_step  :       (p.step h).nodup <-> p.nodup ∧ z ∉ p        := iff.rfl
+        @[simp] lemma mem_step    :            u ∈ (p · h) <-> u ∈ p ∨ u = z    := iff.rfl
+        @[simp] lemma size_step   :           size (p · h)  =  size p + 1       := rfl
+        @[simp] lemma rev_step    :            rev (p · h)  =  h.symm :: p.rev  := rfl
+        @[simp] lemma edges_step  :          edges (p · h)  =  ⟨h⟩ :: edges p   := rfl
+        @[simp] lemma nodup_step  :          nodup (p · h) <-> nodup p ∧ z ∉ p  := iff.rfl
 
         lemma mem_tail : y ∈ p := by { cases p, exact rfl, exact or.inr rfl }
         lemma mem_head : x ∈ p := path.rec rfl (λ _ _ _ _, or.inl) p
 
         lemma point_of_size_0 : p.size = 0 -> x = y := by { intro h, cases p, refl, contradiction }
 
-        @[simp] lemma mem_cons      :            v ∈ p.cons h' <-> v = u ∨ v ∈ p         := by { induction p; simp [*,or.assoc] }
-        @[simp] lemma size_cons     :         size (p.cons h')  =  size p + 1            := by { induction p, obviously }
+        @[simp] lemma mem_cons      :              v ∈ h' :: p <-> v = u ∨ v ∈ p         := by { induction p; simp [*,or.assoc] }
+        @[simp] lemma size_cons     :         size (cons h' p)  =  size p + 1            := by { induction p, obviously }
         @[simp] lemma size_rev      :             size (rev p)  =  size p                := by { induction p, obviously }
         @[simp] lemma mem_rev       :                z ∈ rev p <-> z ∈ p                 := by { induction p; simp [*,or.comm] }
         @[simp] lemma concat_point' :           concat point p  =  p                     := by { induction p, obviously }
-        @[simp] lemma concat_step'  : concat (step point h') p  =  cons p h'             := by { induction p, obviously }
-        @[simp] lemma concat_cons   :    concat (p.cons h') p'  =  cons (concat p p') h' := by { induction p', obviously }
+        @[simp] lemma concat_step'  : concat (step point h') p  =  cons h' p             := by { induction p, obviously }
+        @[simp] lemma concat_cons   :    concat (cons h' p) p'  =  cons h' (concat p p') := by { induction p', obviously }
         @[simp] lemma concat_rev    :        rev (concat p p')  =  concat p'.rev p.rev   := by { induction p', obviously }
         @[simp] lemma size_concat   :       size (concat p p')  =  p.size + p'.size      := by { induction p'; simp [*,add_assoc] }
 
@@ -86,7 +94,7 @@ namespace simple_graph
 
         lemma iff_path : linked G x y <-> nonempty (path G x y) := ⟨to_path, from_path⟩
 
-        @[simp] lemma nodup_cons : nodup (cons p h') <-> u ∉ p ∧ nodup p
+        @[simp] lemma nodup_cons : nodup (cons h' p) <-> u ∉ p ∧ nodup p
             := by { induction p with a b h1 h2 ih, simp, exact ne_comm,
                 simp, push_neg, split,
                 { rintros ⟨h1,h2,h3⟩, have h4 := ih.mp h1, exact ⟨⟨h4.1,h2.symm⟩,h4.2,h3⟩ },
